New, much simpler example

theories/Example.v
@@ -161,192 +161,149 @@ Make Definition coq_realid :=
 
 (*! EXAMPLE 3 *)
 
-Fail Definition vrev {A n m} (v : vec A n) (acc : vec A m) : vec A (n + m) :=
-  vec_rect A (fun n _ => forall m, vec A m -> vec A (n + m)) 
-           (fun m acc => acc) (fun a n _ rv m acc => rv _ (vcons a m acc))
-           n v m acc.
+Fail Definition vcons_act {A n X} (f : vec A (n + 1) -> X) (a : A) (v : vec A n) : X
+  := f (vcons a n v).
 
-Definition vrev {A n m} (v : vec A n) (acc : vec A m) : vec A (n + m) :=
-  vec_rect A (fun n _ => forall m, vec A m -> vec A (n + m)) 
-           (fun m acc => acc) (fun a n _ rv m acc => {! rv _ (vcons a m acc) !})
-           n v m acc.
+Definition vcons_act {A n X} (f : vec A (n + 1) -> X) (a : A) (v : vec A n) : X
+  := f {! vcons a n v !}.
 
-Quote Definition vrev_term :=
-  ltac:(let t := eval unfold vrev in @vrev in exact t).
-Quote Definition vrev_type := 
-  ltac:(let T := type of @vrev in exact T).
+Quote Definition vcons_act_term :=
+  ltac:(let t := eval unfold vcons_act in @vcons_act in exact t).
+Quote Definition vcons_act_type := 
+  ltac:(let T := type of @vcons_act in exact T).
 
-Definition pretm_vrev :=
-  Eval lazy - [Σi] in fullquote (2 ^ 18) Σ [] vrev_term indt constt cot.
-Definition tm_vrev :=
+Definition pretm_vcons_act :=
+  Eval lazy - [Σi] in fullquote (2 ^ 18) Σ [] vcons_act_term indt constt cot.
+Definition tm_vcons_act :=
   Eval lazy - [Σi] in 
-  match pretm_vrev with
+  match pretm_vcons_act with
   | Success t => t
   | Error _ => sRel 0
   end.
 
-Definition prety_vrev :=
-  Eval lazy in fullquote (2 ^ 18) Σ [] vrev_type indt constt cot.
-Definition ty_vrev :=
+Definition prety_vcons_act :=
+  Eval lazy in fullquote (2 ^ 18) Σ [] vcons_act_type indt constt cot.
+Definition ty_vcons_act :=
   Eval lazy in 
-  match prety_vrev with
+  match prety_vcons_act with
   | Success t => t
   | Error _ => sRel 0
   end.
 
-(* TODO Move in ExamplesUtil *)
-Fixpoint Prods (Γ : scontext) (T : sterm) :=
-  match Γ with
-  | A :: Γ => Prods Γ (sProd nAnon A T)
-  | [] => T
-  end.
-
-Lemma lift_rel :
-  forall {t k}, (lift 1 (S k) t) {k := sRel 0} = t.
+Lemma type_vcons_act : Σi ;;; [] |-x tm_vcons_act : ty_vcons_act.
 Proof.
-  intro t. induction t ; intro k.
-  all: try (cbn ; f_equal ; easy).
-  destruct n.
-  - cbn. case_eq (k ?= 0) ; intro e ; bprop e.
-    + subst. reflexivity.
-    + reflexivity.
-    + reflexivity.
-  - cbn. case_eq (k <=? n) ; intro e ; bprop e.
-    + cbn. case_eq (k ?= S (S n)) ; intro e1 ; bprop e1 ; try myomega.
-      reflexivity.
-    + cbn. case_eq (k ?= S n) ; intro e1 ; bprop e1 ; try myomega.
-      * subst. f_equal. myomega.
-      * reflexivity.
-Defined.
-
-Lemma close_goal_ex :
-  forall {Σ Γ t T},
-    xtype_glob Σ ->
-    Σ ;;; [] |-x t : Prods Γ T ->
-    Σ ;;; Γ |-x T : Ty ->
-    ∑ t', Σ ;;; Γ |-x t' : T.
-Proof.
-  intros Σ Γ t T hg h hT.
-  revert t T h hT. induction Γ as [| A Γ].
-  - intros t T h hT. eexists. eassumption.
-  - intros t T h hT. cbn in h.
-    destruct (IHΓ _ _ h) as [t' ht'].
-    + pose proof (typing_wf hT) as hw.
-      inversion hw. subst. destruct s.
-      eapply xtype_Prod'.
-      * eassumption.
-      * intros _. eassumption.
-    + eexists. eapply meta_conv.
-      * eapply xtype_App'.
-        -- assumption.
-        -- instantiate (2 := lift0 1 A).
-           instantiate (1 := lift 1 1 T).
-           instantiate (1 := nAnon).
-           change (sProd nAnon (lift0 1 A) (lift 1 1 T))
-             with (lift0 1 (sProd nAnon A T)).
-           eapply typing_lift01.
-           ++ assumption.
-           ++ exact ht'.
-           ++ instantiate (1 := tt).
-              pose proof (typing_wf hT) as hw.
-              inversion hw. subst. destruct s.
-              assumption.
-        -- instantiate (1 := sRel 0). ettcheck  Σi.
-           pose proof (typing_wf hT) as hw.
-           inversion hw. subst. destruct s.
-           assumption.
-      * eapply lift_rel.
-Defined.
-
-Lemma inversionProds :
-  forall {Σ Γ T},
-    Σ ;;; [] |-x Prods Γ T : Ty ->
-    (Σ ;;; Γ |-x T : Ty).
-Proof.
-  intros Σ Γ T h. revert T h.
-  induction Γ as [| A Γ] ; intros T h.
-  - cbn in h. assumption.
-  - cbn in h.
-    specialize (IHΓ _ h).
-    destruct (XInversions.inversionProd IHΓ) as [[? ?] ?].
-    assumption.
-Defined.
-
-Lemma close_goal_ex' :
-  forall {Σ Γ t T},
-    xtype_glob Σ ->
-    Σ ;;; [] |-x t : Prods Γ T ->
-    ∑ t', Σ ;;; Γ |-x t' : T.
-Proof.
-  intros Σ Γ t T hg ht.
-  eapply close_goal_ex ; try eassumption.
-  destruct (istype_type hg ht) as [[] hT].
-  eapply inversionProds. assumption.
-Defined.
-
-Definition closet {Σ Γ t T} hg h :=
-  let '(t' ; _) := @close_goal_ex' Σ Γ t T hg h in t'.
-
-Definition close_goal :
-  forall {Σ Γ t T}
-    (hg : xtype_glob Σ)
-    (h : Σ ;;; [] |-x t : Prods Γ T),
-    Σ ;;; Γ |-x closet hg h : T.
-Proof.
-  intros Σ Γ t T h.
-  eapply close_goal_ex'.
-Defined.
-
-Transparent Σi.
-
-Lemma type_vrev : Σi ;;; [] |-x tm_vrev : ty_vrev.
-Proof.
-  unfold tm_vrev, ty_vrev.
+  unfold tm_vcons_act, ty_vcons_act.
   pose proof xhΣi.
   ettcheck Σi.
-  - eapply reflection.
-    unshelve eapply close_goal
-    ; [ exact (sAx "vrev_obligation1") | assumption |].
-    simpl. ettcheck Σi. 
-  - eapply reflection.
-    unshelve eapply close_goal
-    ; [ exact (sAx "vrev_obligation2") | assumption |].
-    simpl. ettcheck Σi.
-  - eapply reflection.
-    unshelve eapply close_goal
-    ; [ exact (sAx "vrev_obligation3") | assumption |].
-    simpl. ettcheck Σi.
-  - eapply reflection.
-    unshelve eapply close_goal
-    ; [ exact (sAx "vrev_obligation4") | assumption |].
-    simpl. ettcheck Σi.
-  Unshelve. exact nAnon.
+  eapply reflection.
+  unshelve eapply close_goal
+  ; [ exact (sAx "vcons_act_obligation") | assumption |].
+  simpl. ettcheck Σi.
 Defined.
 
-Definition type_vrev_ := Eval lazy - [Σi] in type_vrev.
-
-Print type_vrev_.
-
-Definition itt_vrev : sterm :=
+Definition itt_vcons_act : sterm :=
   Eval lazy in
-  let '(_ ; t ; _) := type_translation type_vrev_ istrans_nil in t.
+  let '(_ ; t ; _) := type_translation type_vcons_act istrans_nil in t.
 
-Print itt_vrev.
+Print itt_vcons_act.
 
-Definition tc_vrev : tsl_result term :=
+Definition tc_vcons_act : tsl_result term :=
   Eval lazy in
-  tsl_rec (2 ^ 18) Σ [] itt_vrev empty.
+  tsl_rec (2 ^ 18) Σ [] itt_vcons_act empty.
 
-Print tc_vrev.
+Print tc_vcons_act.
 
-Make Definition coq_vrev :=
+Make Definition coq_vcons_act :=
   ltac:(
     let t := eval lazy in
-             (match tc_vrev with
+             (match tc_vcons_act with
               | FinalTranslation.Success _ t => t
               | _ => tRel 0
               end)
       in exact t
   ).
 
-Print coq_vrev.
+Print coq_vcons_act.
+
+(*! EXAMPLE 4 *)
+
+(* Fail Definition vrev {A n m} (v : vec A n) (acc : vec A m) : vec A (n + m) := *)
+(*   vec_rect A (fun n _ => forall m, vec A m -> vec A (n + m))  *)
+(*            (fun m acc => acc) (fun a n _ rv m acc => rv _ (vcons a m acc)) *)
+(*            n v m acc. *)
+
+(* Definition vrev {A n m} (v : vec A n) (acc : vec A m) : vec A (n + m) := *)
+(*   vec_rect A (fun n _ => forall m, vec A m -> vec A (n + m))  *)
+(*            (fun m acc => acc) (fun a n _ rv m acc => {! rv _ (vcons a m acc) !}) *)
+(*            n v m acc. *)
+
+(* Quote Definition vrev_term := *)
+(*   ltac:(let t := eval unfold vrev in @vrev in exact t). *)
+(* Quote Definition vrev_type :=  *)
+(*   ltac:(let T := type of @vrev in exact T). *)
+
+(* Definition pretm_vrev := *)
+(*   Eval lazy - [Σi] in fullquote (2 ^ 18) Σ [] vrev_term indt constt cot. *)
+(* Definition tm_vrev := *)
+(*   Eval lazy - [Σi] in  *)
+(*   match pretm_vrev with *)
+(*   | Success t => t *)
+(*   | Error _ => sRel 0 *)
+(*   end. *)
+
+(* Definition prety_vrev := *)
+(*   Eval lazy in fullquote (2 ^ 18) Σ [] vrev_type indt constt cot. *)
+(* Definition ty_vrev := *)
+(*   Eval lazy in  *)
+(*   match prety_vrev with *)
+(*   | Success t => t *)
+(*   | Error _ => sRel 0 *)
+(*   end. *)
+
+(* Lemma type_vrev : Σi ;;; [] |-x tm_vrev : ty_vrev. *)
+(* Proof. *)
+(*   unfold tm_vrev, ty_vrev. *)
+(*   pose proof xhΣi. *)
+(*   ettcheck Σi. *)
+(*   - eapply reflection. *)
+(*     unshelve eapply close_goal *)
+(*     ; [ exact (sAx "vrev_obligation1") | assumption |]. *)
+(*     simpl. ettcheck Σi.  *)
+(*   - eapply reflection. *)
+(*     unshelve eapply close_goal *)
+(*     ; [ exact (sAx "vrev_obligation2") | assumption |]. *)
+(*     simpl. ettcheck Σi. *)
+(*   - eapply reflection. *)
+(*     unshelve eapply close_goal *)
+(*     ; [ exact (sAx "vrev_obligation3") | assumption |]. *)
+(*     simpl. ettcheck Σi. *)
+(*   - eapply reflection. *)
+(*     unshelve eapply close_goal *)
+(*     ; [ exact (sAx "vrev_obligation4") | assumption |]. *)
+(*     simpl. ettcheck Σi. *)
+(*   Unshelve. exact nAnon. *)
+(* Defined. *)
+
+(* Definition itt_vrev : sterm := *)
+(*   Eval lazy in *)
+(*   let '(_ ; t ; _) := type_translation type_vrev istrans_nil in t. *)
+
+(* (* Print itt_vrev. *) *)
+
+(* Definition tc_vrev : tsl_result term := *)
+(*   Eval lazy in *)
+(*   tsl_rec (2 ^ 18) Σ [] itt_vrev empty. *)
+
+(* (* Print tc_vrev. *) *)
+
+(* Make Definition coq_vrev := *)
+(*   ltac:( *)
+(*     let t := eval lazy in *)
+(*              (match tc_vrev with *)
+(*               | FinalTranslation.Success _ t => t *)
+(*               | _ => tRel 0 *)
+(*               end) *)
+(*       in exact t *)
+(*   ). *)
+
+(* (* Print coq_vrev. *) *)
