theories/ExamplesUtil.v
@@ -49,10 +49,11 @@ Definition glob_term :=
   let _ := vec in
   let _ := vec_rect in
   let _ := Nat.add in
-  let _ := vrev_obligation1 in
-  let _ := vrev_obligation2 in
-  let _ := vrev_obligation3 in
-  let _ := vrev_obligation4 in
+  (* let _ := vrev_obligation1 in *)
+  (* let _ := vrev_obligation2 in *)
+  (* let _ := vrev_obligation3 in *)
+  (* let _ := vrev_obligation4 in *)
+  let _ := vcons_act_obligation in
   Type.
 
 Quote Recursively Definition glob_prog := @glob_term.
@@ -165,16 +166,16 @@ Definition ty_vcons :=
   end.
 
 (* vec_rect *)
-Quote Definition vec_rect_type :=
-  ltac:(let T := type of @vec_rect in exact T).
-Definition prety_vec_rect :=
-  Eval lazy in fullquote (2 ^ 18) Σ [] vec_rect_type indt constt cot.
-Definition ty_vec_rect :=
-  Eval lazy in
-  match prety_vec_rect with
-  | Success t => t
-  | Error _ => sRel 0
-  end.
+(* Quote Definition vec_rect_type := *)
+(*   ltac:(let T := type of @vec_rect in exact T). *)
+(* Definition prety_vec_rect := *)
+(*   Eval lazy in fullquote (2 ^ 18) Σ [] vec_rect_type indt constt cot. *)
+(* Definition ty_vec_rect := *)
+(*   Eval lazy in *)
+(*   match prety_vec_rect with *)
+(*   | Success t => t *)
+(*   | Error _ => sRel 0 *)
+(*   end. *)
 
 (* add *)
 Quote Definition add_type :=
@@ -192,12 +193,13 @@ Definition ty_add :=
 (* The global context *)
 
 Definition Σi : sglobal_context := [
-  decl "vrev_obligation4" ty_obligation4 ;
-  decl "vrev_obligation3" ty_obligation3 ;
-  decl "vrev_obligation2" ty_obligation2 ;
-  decl "vrev_obligation1" ty_obligation1 ;
+  (* decl "vrev_obligation4" ty_obligation4 ; *)
+  (* decl "vrev_obligation3" ty_obligation3 ; *)
+  (* decl "vrev_obligation2" ty_obligation2 ; *)
+  (* decl "vrev_obligation1" ty_obligation1 ; *)
+  decl "vcons_act_obligation" ty_vcons_act_obligation ;
   decl "add" ty_add ;
-  decl "vec_rect" ty_vec_rect ;
+  (* decl "vec_rect" ty_vec_rect ; *)
   decl "vcons" ty_vcons ;
   decl "vnil" ty_vnil ;
   decl "vec" ty_vec ;
@@ -229,10 +231,11 @@ Proof.
   - ittcheck_env.
   - ittcheck_env.
   - ittcheck_env.
-  - ittcheck_env.
-  - ittcheck_env.
-  - ittcheck_env.
-  - ittcheck_env.
+  (* - ittcheck_env. *)
+  (* - ittcheck_env. *)
+  (* - ittcheck_env. *)
+  (* - ittcheck_env. *)
+  (* - ittcheck_env. *)
   - ittcheck_env.
   Unshelve. all: exact nAnon.
 Defined.
@@ -252,10 +255,11 @@ Proof.
   - ettcheck_env.
   - ettcheck_env.
   - ettcheck_env.
-  - ettcheck_env.
-  - ettcheck_env.
-  - ettcheck_env.
-  - ettcheck_env.
+  (* - ettcheck_env. *)
+  (* - ettcheck_env. *)
+  (* - ettcheck_env. *)
+  (* - ettcheck_env. *)
+  (* - ettcheck_env. *)
   - ettcheck_env.
   Unshelve. all: exact nAnon.
 Defined.
@@ -270,3 +274,108 @@ Defined.
 
 Definition type_translation {Γ t A} h {Γ'} hΓ :=
   pi2_ (pi1_ (@complete_translation _ Σi hΣi)) Γ t A h Γ' hΓ.
+
+
+
+(* Useful lemmata *)
+Fixpoint Prods (Γ : scontext) (T : sterm) :=
+  match Γ with
+  | A :: Γ => Prods Γ (sProd nAnon A T)
+  | [] => T
+  end.
+
+Lemma lift_rel :
+  forall {t k}, (lift 1 (S k) t) {k := sRel 0} = t.
+Proof.
+  intro t. induction t ; intro k.
+  all: try (cbn ; f_equal ; easy).
+  destruct n.
+  - cbn. case_eq (k ?= 0) ; intro e ; bprop e.
+    + subst. reflexivity.
+    + reflexivity.
+    + reflexivity.
+  - cbn. case_eq (k <=? n) ; intro e ; bprop e.
+    + cbn. case_eq (k ?= S (S n)) ; intro e1 ; bprop e1 ; try myomega.
+      reflexivity.
+    + cbn. case_eq (k ?= S n) ; intro e1 ; bprop e1 ; try myomega.
+      * subst. f_equal. myomega.
+      * reflexivity.
+Defined.
+
+Lemma close_goal_ex :
+  forall {Σ Γ t T},
+    xtype_glob Σ ->
+    Σ ;;; [] |-x t : Prods Γ T ->
+    Σ ;;; Γ |-x T : Ty ->
+    ∑ t', Σ ;;; Γ |-x t' : T.
+Proof.
+  intros Σ Γ t T hg h hT.
+  revert t T h hT. induction Γ as [| A Γ].
+  - intros t T h hT. eexists. eassumption.
+  - intros t T h hT. cbn in h.
+    destruct (IHΓ _ _ h) as [t' ht'].
+    + pose proof (typing_wf hT) as hw.
+      inversion hw. subst. destruct s.
+      eapply xtype_Prod'.
+      * eassumption.
+      * intros _. eassumption.
+    + eexists. eapply meta_conv.
+      * eapply xtype_App'.
+        -- assumption.
+        -- instantiate (2 := lift0 1 A).
+           instantiate (1 := lift 1 1 T).
+           instantiate (1 := nAnon).
+           change (sProd nAnon (lift0 1 A) (lift 1 1 T))
+             with (lift0 1 (sProd nAnon A T)).
+           eapply typing_lift01.
+           ++ assumption.
+           ++ exact ht'.
+           ++ instantiate (1 := tt).
+              pose proof (typing_wf hT) as hw.
+              inversion hw. subst. destruct s.
+              assumption.
+        -- instantiate (1 := sRel 0). ettcheck  Σi.
+           pose proof (typing_wf hT) as hw.
+           inversion hw. subst. destruct s.
+           assumption.
+      * eapply lift_rel.
+Defined.
+
+Lemma inversionProds :
+  forall {Σ Γ T},
+    Σ ;;; [] |-x Prods Γ T : Ty ->
+    (Σ ;;; Γ |-x T : Ty).
+Proof.
+  intros Σ Γ T h. revert T h.
+  induction Γ as [| A Γ] ; intros T h.
+  - cbn in h. assumption.
+  - cbn in h.
+    specialize (IHΓ _ h).
+    destruct (XInversions.inversionProd IHΓ) as [[? ?] ?].
+    assumption.
+Defined.
+
+Lemma close_goal_ex' :
+  forall {Σ Γ t T},
+    xtype_glob Σ ->
+    Σ ;;; [] |-x t : Prods Γ T ->
+    ∑ t', Σ ;;; Γ |-x t' : T.
+Proof.
+  intros Σ Γ t T hg ht.
+  eapply close_goal_ex ; try eassumption.
+  destruct (istype_type hg ht) as [[] hT].
+  eapply inversionProds. assumption.
+Defined.
+
+Definition closet {Σ Γ t T} hg h :=
+  let '(t' ; _) := @close_goal_ex' Σ Γ t T hg h in t'.
+
+Definition close_goal :
+  forall {Σ Γ t T}
+    (hg : xtype_glob Σ)
+    (h : Σ ;;; [] |-x t : Prods Γ T),
+    Σ ;;; Γ |-x closet hg h : T.
+Proof.
+  intros Σ Γ t T h.
+  eapply close_goal_ex'.
+Defined.
